chore: dont allow changing viewing key
commit-id:10805e22

lean/privacy/channels/discoverable.lean
@@ -4,9 +4,8 @@ import privacy.channels.channels
 import privacy.channels.contiguous
 
 def scan_channels (crypto: Crypto) (m: Memory) (addrbob: ℕ) (kbob: crypto.PrivateKeys) : List ℕ :=
-  let Kbob := crypto.priv_to_pub kbob
-  let num_channels := m .ChannelsJ [addrbob, Kbob]
-  List.range num_channels |>.map (λ j ↦ (crypto.dec kbob (m .Channels [addrbob, Kbob, j])).headD 0)
+  let num_channels := m .ChannelsJ [addrbob]
+  List.range num_channels |>.map (λ j ↦ (crypto.dec kbob (m .Channels [addrbob, j])).headD 0)
 
 theorem scan_channels_monotone
    {crypto: Crypto} {m: Memory} {addrbob c: ℕ} {kbob: crypto.PrivateKeys}
@@ -24,10 +23,10 @@ theorem scan_channels_monotone
 
     generalize h_Kbob: crypto.priv_to_pub kbob = Kbob at *
 
-    by_cases h_bob: addrbob = inp.addrbob ∧ Kbob = inp.Kbob
+    by_cases h_bob: addrbob = inp.addrbob
     case pos =>
-      rw [h_bob.1, h_bob.2] at h
-      rw [h_bob.1, h_bob.2]
+      rw [h_bob] at h
+      rw [h_bob]
       constructor
       · rw [info.memory_diff₀]; omega
       · by_cases h_j': j = info.j
@@ -37,11 +36,50 @@ theorem scan_channels_monotone
           exact h.2
     case neg =>
       rw [info.no_change _ _ (by simp [h_bob])]
-      have : ¬(addrbob = inp.addrbob ∧ Kbob = inp.Kbob ∧ j = info.j) := λ h ↦ h_bob ⟨h.1, h.2.1⟩
+      have : ¬(addrbob = inp.addrbob ∧ j = info.j) := λ h ↦ h_bob h.1
       rw [info.no_change _ _ (by simp [this])]
       exact h
 
   all_goals exact h
+
+-- If bob was not registered, then scan_channels will return an empty list.
+theorem channels_j_zero
+    {crypto: Crypto} {rm: ReachableMemory crypto} {addrbob: ℕ}
+    (h: rm.m .PublicKeys [addrbob] = 0) :
+    rm.m .ChannelsJ [addrbob] = 0  := by
+  revert rm
+  apply ReachableMemory.induction
+
+  case inv₀ => intro h; trivial
+
+  intro action rm ih success h
+  cases action
+  case CreateChannel inp =>
+    let info := create_channel_info crypto inp rm success
+    rw [ReachableMemory.add_m, run_action, ←info.h_m'] at h ⊢
+    rw [info.no_change _ _ (by simp)] at h
+    by_cases h_bob: addrbob = inp.addrbob
+    case pos =>
+      rw [h_bob] at h
+      have := info.h_Kbob ▸ info.bob_registered
+      contradiction
+    case neg =>
+      rw [info.no_change _ _ (by simp [h_bob])]
+      exact ih h
+
+  case Register inp =>
+    let info := register_info crypto inp rm success
+    rw [ReachableMemory.add_m, run_action, ←info.h_m'] at h ⊢
+    rw [info.no_change _ _ (by simp)]
+    by_cases h_bob: addrbob = inp.addralice
+    case pos =>
+      rw [h_bob] at ih ⊢
+      exact ih info.alice_was_not_registered
+    case neg =>
+      rw [info.no_change _ _ (by simp [h_bob])] at h
+      exact ih h
+
+  all_goals exact ih h
 
 -----------------------------------------
 -- Channel exists implies discoverable --
@@ -79,7 +117,6 @@ theorem channels_are_discoverable {crypto: Crypto} {rm: ReachableMemory crypto} 
         injections h₀
       · simp only [scan_channels]
         simp only [List.headD_eq_head?_getD, List.mem_map, List.mem_range]
-        rw [h_Kbob]
         use info.j
         constructor
         · rw [info.h_j, info.memory_diff₀]; omega
@@ -96,13 +133,14 @@ theorem channels_are_discoverable {crypto: Crypto} {rm: ReachableMemory crypto} 
 
 -- Discoverable channel → channel_exists and c is linked to (addrbob, kbob).
 theorem discoverable_channel_implies_exists
-    (crypto: Crypto) (rm: ReachableMemory crypto) (addrbob: ℕ) (kbob: crypto.PrivateKeys) (c: ℕ)
+    {crypto: Crypto} {rm: ReachableMemory crypto} {addrbob: ℕ} {kbob: crypto.PrivateKeys} {c: ℕ}
+    (k_kbob: rm.m .PublicKeys [addrbob] = crypto.priv_to_pub kbob)
     (h: c ∈ scan_channels crypto rm addrbob kbob) :
     channel_exists crypto rm c ∧
     ∃ addralice kalice, c = crypto.hash [addralice, kalice, addrbob, crypto.priv_to_pub kbob] := by
   revert rm
   apply ReachableMemory.induction
-  case inv₀ => intro h; trivial
+  case inv₀ => intro h_kbob h; trivial
 
   intro action rm ih success
 
@@ -110,18 +148,21 @@ theorem discoverable_channel_implies_exists
   case CreateChannel inp =>
     let info := create_channel_info crypto inp rm success
     rw [ReachableMemory.add_m, run_action, ←info.h_m'] at *
-    intro channel_discoverable_
+    intro h_kbob h_channel_discoverable
     simp only [scan_channels, List.headD_eq_head?_getD, List.mem_map, List.mem_range] at *
-    obtain ⟨j, j_lt, channel_decryption⟩ := channel_discoverable_
-    by_cases h_bob: addrbob = inp.addrbob ∧ crypto.priv_to_pub kbob = inp.Kbob
+    obtain ⟨j, j_lt, channel_decryption⟩ := h_channel_discoverable
+    by_cases h_bob: addrbob = inp.addrbob
     case pos =>
-      rw [h_bob.1, h_bob.2] at j_lt ih channel_decryption
+      rw [h_bob] at j_lt ih channel_decryption
       rw [info.memory_diff₀] at j_lt
       rw [←info.h_j] at *
+      rw [info.no_change _ _ (by simp), h_bob] at h_kbob
+      have h_Kbob : inp.Kbob = crypto.priv_to_pub kbob := by
+        rw [←info.h_Kbob, h_kbob]
       by_cases same_j: j = info.j
       case pos =>
         have h_c : c = inp.c crypto := by
-          rw [same_j, info.memory_diff₁, CreateChannelInput.enc, ←h_bob.2, crypto.dec_enc] at channel_decryption
+          rw [same_j, info.memory_diff₁, CreateChannelInput.enc, h_Kbob, crypto.dec_enc] at channel_decryption
           simp at channel_decryption
           simp [channel_decryption]
         constructor
@@ -129,18 +170,34 @@ theorem discoverable_channel_implies_exists
           use inp.addralice, inp.addrbob, inp.Kbob
           simp [h_c, info.memory_diff₂]
         · use inp.addralice, inp.kalice
-          rw [h_c, h_bob.1, h_bob.2]
+          rw [h_c, ←h_Kbob, h_bob]
       case neg =>
         rw [info.no_change _ _ (by simp [same_j])] at channel_decryption
-        have ⟨h₀, h₁⟩ := ih ⟨j, (by omega), channel_decryption⟩
-        rw [h_bob.1, h_bob.2, info.h_m']
+        have ⟨h₀, h₁⟩ := ih h_kbob ⟨j, (by omega), channel_decryption⟩
+        rw [h_bob, info.h_m']
         use channel_exists_monotone crypto rm (.CreateChannel inp) c success h₀
     case neg =>
       rw [info.no_change _ _ (by simp [h_bob])] at j_lt
-      have : ¬(addrbob = inp.addrbob ∧ crypto.priv_to_pub kbob = inp.Kbob ∧ j = info.j) := λ h ↦ h_bob ⟨h.1, h.2.1⟩
+      have : ¬(addrbob = inp.addrbob ∧ j = info.j) := λ h ↦ h_bob h.1
       rw [info.no_change _ _ (by simp [this])] at channel_decryption
-      have ⟨h₀, h₁⟩ := ih ⟨j, j_lt, channel_decryption⟩
+      rw [info.no_change _ _ (by simp)] at h_kbob
+      have ⟨h₀, h₁⟩ := ih h_kbob ⟨j, j_lt, channel_decryption⟩
       rw [info.h_m']
       use channel_exists_monotone crypto rm (.CreateChannel inp) c success h₀
+
+  case Register inp =>
+    intro h_kbob h_channel_discoverable
+    let info := register_info crypto inp rm success
+    rw [ReachableMemory.add_m, run_action, ←info.h_m'] at h_kbob
+    by_cases same_addrbob: addrbob = inp.addralice
+    case pos =>
+      have : (rm.add (.Register inp) success).m MemoryType.ChannelsJ [inp.addralice] = 0 := by
+        rw [ReachableMemory.add_m, run_action, ←info.h_m', info.no_change _ _ (by simp)]
+        exact channels_j_zero info.alice_was_not_registered
+      rw [scan_channels, same_addrbob, this] at h_channel_discoverable
+      simp at h_channel_discoverable
+    case neg =>
+      rw [info.no_change _ _ (by simp [same_addrbob])] at h_kbob
+      exact ih h_kbob h_channel_discoverable
 
   all_goals exact ih
